ictr.fst
@@ -1,6 +1,8 @@
 module Ictr
 open FStar.List.Tot
 
+#set-options "--query_stats"
+
 open Library
 
 type s = nat
@@ -13,12 +15,12 @@ type op = |Add
 
 let init = 0
 
-let pre_cond_app_op s1 op = true
-let pre_cond_prop_oper tr s1 op = true
+let pre_cond_do s1 op = true
+let pre_cond_prop_do tr s1 op = true
 
-val app_op : s1:s -> op:(nat * op) -> Tot (s2:(s * rval) {get_op op = Add ==> s2 = (s1 + 1, Bot) /\
-                                                      get_op op = Rd ==> s2 = (s1, Val s1)})
-let app_op s op1 =
+val do : s1:s -> op:(nat * op) -> Tot (s2:(s * rval) {get_op op = Add ==> s2 = (s1 + 1, Bot) /\
+                                                  get_op op = Rd ==> s2 = (s1, Val s1)})
+let do s op1 =
   match op1 with
   |(_,Add) -> (s + 1, Bot)
   |(_,Rd) -> (s, Val s)
@@ -37,35 +39,54 @@ let spec o tr =
   |(_, Add) -> Bot
   |(_, Rd) -> Val (sum tr.l)
 
-#set-options "--query_stats"
 val sim : tr:ae op
         -> s1:s
         -> Tot (b:bool {b = true <==> (s1 = sum tr.l)})
 let sim tr s1 = (s1 = sum tr.l)
 
+val lemma11 : l:list(nat * op) {unique_id l}
+            -> a:list(nat * op) {unique_id a}
+            -> Lemma (requires (forall e. mem e l ==> not (mem_id (get_id e) a)))
+                    (ensures (sum (union1 l a) = sum l + sum a))
+let rec lemma11 l a =
+  match l,a with
+  |[],[] -> ()
+  |x::xs,_ -> lemma11 xs a
+  |[],_ -> ()
+
 val lemma1 : l:ae op
            -> a:ae op
            -> Lemma (requires (forall e. mem e l.l ==> not (mem_id (get_id e) a.l)))
-                   (ensures (forall e. mem e (union1 l a) <==> mem e l.l \/ mem e a.l) /\
+                   (ensures (forall e. mem e (union l a).l <==> mem e l.l \/ mem e a.l) /\
                             (sum (union l a).l = sum l.l + sum a.l))
-                            (decreases %[l.l;a.l])
-                            [SMTPat (union l a)]
-#set-options "--z3rlimit 1000000"
-let rec lemma1 l a =
-  match l,a with
-  |(A _ []), (A _ []) -> ()
-  |(A _ (x::xs)), _ -> lemma1 (A l.vis xs) a
-  |(A _ []), (A _ (x::xs)) -> lemma1 l (A a.vis xs)
+let lemma1 l a = lemma11 l.l a.l
 
 let pre_cond_merge l a b = a >= l && b >= l
 
 let pre_cond_prop_merge ltr l atr a btr b = true
 
 val merge : l:s -> a:s -> b:s
-           -> Pure s
-             (requires pre_cond_merge l a b)
-             (ensures (fun r -> r = a + b - l))
+          -> Pure s
+            (requires pre_cond_merge l a b)
+            (ensures (fun r -> r = a + b - l))
 let merge l a b = a + b - l
+
+val lemma21 : l:list(nat * op) {unique_id l}
+            -> a:list(nat * op) {unique_id a}
+            -> b:list(nat * op) {unique_id b}
+            -> Lemma (requires (forall e. mem e l ==> not (mem_id (get_id e) a)) /\
+                              (forall e. mem e a ==> not (mem_id (get_id e) b)) /\
+                              (forall e. mem e l ==> not (mem_id (get_id e) b)))
+                    (ensures (forall e. mem e (abs_merge1 l a b) <==> mem e l \/ mem e a \/ mem e b) /\
+                             (sum (abs_merge1 l a b) = sum a + sum b + sum l))
+                             (decreases %[l;a;b])
+#set-options "--z3rlimit 1000"
+let rec lemma21 l a b =
+  match l,a,b with
+  |[],[],[] -> ()
+  |x::xs,_,_ -> lemma21 xs a b
+  |[],x::xs,_ -> lemma21 [] xs b
+  |[],[],_ -> ()
 
 val lemma2 : l:ae op
            -> a:ae op
@@ -73,16 +94,9 @@ val lemma2 : l:ae op
            -> Lemma (requires (forall e. mem e l.l ==> not (mem_id (get_id e) a.l)) /\
                              (forall e. mem e a.l ==> not (mem_id (get_id e) b.l)) /\
                              (forall e. mem e l.l ==> not (mem_id (get_id e) b.l)))
-                   (ensures (forall e. mem e (absmerge1 l a b) <==> mem e l.l \/ mem e a.l \/ mem e b.l) /\
-                            (sum (absmerge l a b).l = sum a.l + sum b.l + sum l.l))
-                            (decreases %[l.l;a.l;b.l])
-                            [SMTPat (sum (absmerge l a b).l)]
-let rec lemma2 l a b =
-  match l,a,b with
-  |(A _ []), (A _ []), (A _ []) -> ()
-  |(A _ (x::xs)), _, _ -> lemma2 (A l.vis xs) a b
-  |(A _ []), (A _ (x::xs)), _ -> lemma2 l (A a.vis xs) b
-  |(A _ []), (A _ []), (A _ (x::xs)) -> lemma2 l a (A b.vis xs)
+                   (ensures (forall e. mem e (abs_merge l a b).l <==> mem e l.l \/ mem e a.l \/ mem e b.l) /\
+                            (sum (abs_merge l a b).l = sum a.l + sum b.l + sum l.l))
+let lemma2 l a b = lemma21 l.l a.l b.l
 
 val prop_merge : ltr:ae op
                -> l:s
@@ -94,7 +108,7 @@ val prop_merge : ltr:ae op
                                  (forall e. mem e atr.l ==> not (mem_id (get_id e) btr.l)) /\
                                  (forall e. mem e ltr.l ==> not (mem_id (get_id e) btr.l)) /\
                                  (sim ltr l /\ sim (union ltr atr) a /\ sim (union ltr btr) b))
-                       (ensures (sim (absmerge ltr atr btr) (merge l a b)))
+                       (ensures (pre_cond_merge l a b) /\ (sim (abs_merge ltr atr btr) (merge l a b)))
 #set-options "--z3rlimit 10000000"
 let prop_merge ltr l atr a btr b = 
   lemma1 ltr atr; 
@@ -102,13 +116,13 @@ let prop_merge ltr l atr a btr b =
   lemma2 ltr atr btr;
   ()
 
-val prop_oper : tr:ae op
-              -> st:s
-              -> op:(nat * op)
-              -> Lemma (requires (sim tr st) /\ (not (mem_id (get_id op) tr.l)) /\
-                                (forall e. mem e tr.l ==> get_id e < get_id op) /\ get_id op > 0)
-                      (ensures (sim (append tr op) (get_st (app_op st op))))
-let prop_oper tr st op = ()
+val prop_do : tr:ae op
+            -> st:s
+            -> op:(nat * op)
+            -> Lemma (requires (sim tr st) /\ (not (mem_id (get_id op) tr.l)) /\
+                              (forall e. mem e tr.l ==> get_id e < get_id op) /\ get_id op > 0)
+                    (ensures (sim (abs_do tr op) (get_st (do st op))))
+let prop_do tr st op = ()
 
 val convergence : tr:ae op
                 -> a:s
@@ -122,20 +136,20 @@ val prop_spec : tr:ae op
               -> op:(nat * op)
               -> Lemma (requires (sim tr st) /\ (not (mem_id (get_id op) tr.l)) /\
                                 (forall e. mem e tr.l ==> get_id e < get_id op) /\ get_id op > 0)
-                      (ensures (get_rval (app_op st op) = spec op tr))
+                      (ensures (get_rval (do st op) = spec op tr))
 let prop_spec tr st op = ()
 
 instance ictr : mrdt s op rval = {
   Library.init = init;
   Library.spec = spec;
   Library.sim = sim;
-  Library.pre_cond_app_op = pre_cond_app_op;
-  Library.pre_cond_prop_oper = pre_cond_prop_oper;
+  Library.pre_cond_do = pre_cond_do;
+  Library.pre_cond_prop_do = pre_cond_prop_do;
   Library.pre_cond_merge = pre_cond_merge;
   Library.pre_cond_prop_merge = pre_cond_prop_merge;
-  Library.app_op = app_op;
+  Library.do = do;
   Library.merge = merge;
-  Library.prop_oper = prop_oper;
+  Library.prop_do = prop_do;
   Library.prop_merge = prop_merge;
   Library.prop_spec = prop_spec;
   Library.convergence = convergence
