log.fst
@@ -1,6 +1,8 @@
 module Log
 open FStar.List.Tot
 
+#set-options "--query_stats"
+
 open Library
 
 val fst : e:(nat * string) -> Tot (id:nat {exists m. e = (id, m)})
@@ -37,26 +39,11 @@ let rec total_order l =
   |[x] -> true
   |x::xs ->  forallb (fun e -> fst x > fst e) xs && total_order xs
 
-val test_sorted : x:(nat * string) -> l:list (nat * string) 
-                -> Lemma ((unique_s (x::l) /\ total_order (x::l) /\ Cons? l) ==> fst x > fst (Cons?.hd l))
-let test_sorted x l = ()
-
 val ord : id:(nat * string)
         -> id1:(nat * string) {fst id <> fst id1}
         -> l:list (nat * string) {mem id l /\ mem id1 l /\ unique_s l /\ total_order l}
         -> Tot (b:bool {b = true <==> pos id l < pos id1 l})
 let ord id id1 l = pos id l < pos id1 l 
-
-val sorted_smaller : x:(nat * string)
-                   -> y:(nat * string)
-                   -> l:list (nat * string)
-                   -> Lemma (requires (unique_s (x::l) /\ total_order (x::l) /\ mem y l))
-                           (ensures (fst x > fst y) /\ ord x y (x::l))
-
-#set-options "--z3rlimit 1000000"
-let rec sorted_smaller x y l = match l with
-  |[] -> ()
-  |z::zs -> if z=y then () else sorted_smaller x y zs
 
 type s = l:list (nat (*timestamp*) * string (*message*)) {unique_s l /\ total_order l}
 
@@ -78,11 +65,10 @@ val filter_uni : f:((nat * string) -> bool)
                -> Lemma (requires (unique_s l /\ total_order l))
                        (ensures (unique_s (filter_s f l) /\ total_order (filter_s f l)) /\
                                  (forall e. mem e l /\ f e <==> mem e (filter_s f l)) /\
-                          (forall e e1. mem e l /\ mem e1 l /\ f e /\ f e1 /\ fst e <> fst e1 /\ fst e > fst e1 /\ ord e e1 l <==>
-       mem e (filter_s f l) /\ mem e1 (filter_s f l) /\ fst e <> fst e1 /\ fst e > fst e1 /\ ord e e1 (filter_s f l)))
+                          (forall e e1. mem e l /\ mem e1 l /\ f e /\ f e1 /\ fst e > fst e1 /\ ord e e1 l <==>
+       mem e (filter_s f l) /\ mem e1 (filter_s f l) /\ fst e > fst e1 /\ ord e e1 (filter_s f l)))
                                [SMTPat (filter_s f l)]
 
-#set-options "--z3rlimit 1000000"
 let rec filter_uni f l =
   match l with
   |[] -> ()
@@ -101,26 +87,25 @@ match o with
 val get_msg : op1:(nat * op){opa op1} -> Tot (s:string {exists id. op1 = (id, (Append s))}) 
 let get_msg (id, (Append m)) = m
 
-val pre_cond_app_op : s1:s
+val pre_cond_do : s1:s
                 -> op1:(nat * op)
                 -> Tot (b:bool {b=true <==> not (mem_id_s (get_id op1) s1) /\ (forall id. mem_id_s id s1 ==> get_id op1 > id)})
-let pre_cond_app_op s1 op = 
+let pre_cond_do s1 op = 
   not (mem_id_s (get_id op) s1) && 
   forallb (fun e -> get_id op > fst e) s1
 
-let pre_cond_prop_oper tr s1 op1 = true
+let pre_cond_prop_do tr s1 op1 = true
 
-val app_op : s1:s
-           -> op1:(nat * op)
-           -> Pure (s * rval)
-             (requires pre_cond_app_op s1 op1)
-             (ensures (fun r -> (opa op1 ==> (forall e. mem e (get_st r) <==> mem e s1 \/ e = (get_id op1, get_msg op1)) /\
-                             (forall e e1. mem e s1 /\ mem e1 s1 /\ fst e <> fst e1 /\ fst e > fst e1 /\ ord e e1 s1 <==>
-                                      mem e (get_st r) /\ mem e1 (get_st r) /\ fst e <> fst e1 /\ fst e > fst e1 /\
-                             e <> (get_id op1, get_msg op1) /\ e1 <> (get_id op1, get_msg op1) /\ ord e e1 (get_st r))) /\
-                             (not (opa op1) ==> r = (s1, Val s1))))
-#set-options "--z3rlimit 1000000"
-let app_op s1 o =
+val do : s1:s
+       -> op1:(nat * op)
+       -> Pure (s * rval)
+         (requires pre_cond_do s1 op1)
+         (ensures (fun r -> (opa op1 ==> (forall e. mem e (get_st r) <==> mem e s1 \/ e = (get_id op1, get_msg op1)) /\
+                         (forall e e1. mem e s1 /\ mem e1 s1 /\ fst e > fst e1 /\ ord e e1 s1 <==>
+                                  mem e (get_st r) /\ mem e1 (get_st r) /\ fst e > fst e1 /\
+                         e <> (get_id op1, get_msg op1) /\ e1 <> (get_id op1, get_msg op1) /\ ord e e1 (get_st r))) /\
+                         (not (opa op1) ==> r = (s1, Val s1))))
+let do s1 o =
   match o with
   |(id, (Append m)) -> ((id, m)::s1, Bot)
   |(_, Rd) -> (s1, Val s1)
@@ -148,45 +133,42 @@ let extract (Val s) = s
 
 assume val spec : o:(nat * op) -> tr:ae op
                 -> Tot (r:rval {(not (opa o) ==> r <> Bot /\ (forall e. mem e (extract r) <==> mem (fst e, (Append (snd e))) tr.l) /\
-                   (forall e e1. mem e (extract r) /\ mem e1 (extract r) /\ fst e <> fst e1 /\ fst e > fst e1 /\ ord e e1 (extract r) <==> mem (fst e, (Append (snd e))) tr.l /\ mem (fst e1, (Append (snd e1))) tr.l /\ fst e <> fst e1 /\ fst e > fst e1 )) /\
+                   (forall e e1. mem e (extract r) /\ mem e1 (extract r) /\ fst e > fst e1 /\ ord e e1 (extract r) <==> mem (fst e, (Append (snd e))) tr.l /\ mem (fst e1, (Append (snd e1))) tr.l /\ fst e > fst e1 )) /\
                             (opa o ==> r = Bot)})
 
-#set-options "--query_stats"
 val sim : tr:ae op
         -> s1:s
         -> Tot (b:bool {b = true <==> (forall e. mem e s1 <==> mem (fst e, (Append (snd e))) tr.l) /\
                                    (forall e e1. (mem (fst e, (Append (snd e))) tr.l /\ 
-                                          mem (fst e1, (Append (snd e1))) tr.l /\ fst e <> fst e1 /\ fst e > fst e1) <==>
-                                          mem e s1 /\ mem e1 s1 /\ fst e <> fst e1 /\ fst e > fst e1 /\ ord e e1 s1)})
+                                          mem (fst e1, (Append (snd e1))) tr.l /\ fst e > fst e1) <==>
+                                          mem e s1 /\ mem e1 s1 /\ fst e > fst e1 /\ ord e e1 s1)})
 
-#set-options "--z3rlimit 1000000"
+#set-options "--z3rlimit 1000"
 let sim tr s1 =
   forallb (fun e -> mem (fst e, (Append (snd e))) tr.l) s1 &&
   forallo (fun e -> opa e && mem (get_id e, get_msg e) s1) (filter (fun e1 -> opa e1) tr.l) &&
   forallb (fun e -> (forallb (fun e1 -> (mem (fst e, (Append (snd e))) tr.l && mem (fst e1, (Append (snd e1))) tr.l &&
-              fst e <> fst e1 && fst e > fst e1))
-  (filter_s (fun e1 -> mem e1 s1 && mem e s1 && fst e <> fst e1 && fst e > fst e1 && ord e e1 s1) s1))) s1 &&
-  forallo (fun e -> opa e && (forallo (fun e1 -> opa e && opa e1 && mem (get_id e, get_msg e) s1 && mem (get_id e1, get_msg e1) s1 && get_id e <> get_id e1 && get_id e > get_id e1 && ord (get_id e, get_msg e) (get_id e1, get_msg e1) s1)
-   (filter (fun e1 -> opa e && opa e1 && (get_id e <> get_id e1 && get_id e > get_id e1)) (filter (fun e1 -> opa e1) tr.l)))) (filter (fun e1 -> opa e1) tr.l)
+              fst e > fst e1))
+  (filter_s (fun e1 -> mem e1 s1 && mem e s1 && fst e > fst e1 && ord e e1 s1) s1))) s1 &&
+  forallo (fun e -> opa e && (forallo (fun e1 -> opa e && opa e1 && mem (get_id e, get_msg e) s1 && mem (get_id e1, get_msg e1) s1 && get_id e > get_id e1 && ord (get_id e, get_msg e) (get_id e1, get_msg e1) s1)
+   (filter (fun e1 -> opa e && opa e1 && get_id e > get_id e1) (filter (fun e1 -> opa e1) tr.l)))) (filter (fun e1 -> opa e1) tr.l)
 
-val prop_oper : tr:ae op
-              -> st:s
-              -> op:(nat * op)
-              -> Lemma (requires (sim tr st) /\ (not (mem_id (get_id op) tr.l)) /\
-                                (forall e. mem e tr.l ==> get_id e < get_id op) /\ get_id op > 0)
-                      (ensures (sim (append tr op) (get_st (app_op st op))))
+val prop_do : tr:ae op
+            -> st:s
+            -> op:(nat * op)
+            -> Lemma (requires (sim tr st) /\ (not (mem_id (get_id op) tr.l)) /\
+                              (forall e. mem e tr.l ==> get_id e < get_id op) /\ get_id op > 0)
+                    (ensures (sim (abs_do tr op) (get_st (do st op))))
 
-#set-options "--z3rlimit 1000000"
-let prop_oper tr st op = ()
+#set-options "--z3rlimit 1000"
+let prop_do tr st op = ()
 
 val remove_st : ele:(nat * string) -> a:s
               -> Pure s
                 (requires (mem ele a))
                 (ensures (fun r -> (forall e. mem e r <==> mem e a /\ e <> ele) /\
-                                (forall e e1. mem e r /\ mem e1 r /\ fst e <> fst e1 /\ ord e e1 r /\ fst e > fst e1 <==>
-                         mem e a /\ mem e1 a /\ fst e <> fst e1 /\ e <> ele /\ e1 <> ele /\ fst e > fst e1 /\ ord e e1 a)))
-
-#set-options "--z3rlimit 1000000"
+                                (forall e e1. mem e r /\ mem e1 r /\ ord e e1 r /\ fst e > fst e1 <==>
+                         mem e a /\ mem e1 a /\ e <> ele /\ e1 <> ele /\ fst e > fst e1 /\ ord e e1 a)))
 let remove_st ele a = filter_s (fun e -> e <> ele) a
 
 val convergence1 : tr:ae op
@@ -194,8 +176,8 @@ val convergence1 : tr:ae op
                  -> b:s
                  -> Lemma (requires (sim tr a /\ sim tr b))
                          (ensures (forall id. mem_id_s id a <==> mem_id_s id b) /\ (forall e. mem e a <==> mem e b) /\
-                                  (forall e e1. mem e a /\ mem e1 a /\ fst e <> fst e1 /\ fst e > fst e1 /\ ord e e1 a <==> 
-                                           mem e b /\ mem e1 b /\ fst e <> fst e1 /\ fst e > fst e1 /\ ord e e1 b))
+                                  (forall e e1. mem e a /\ mem e1 a /\ fst e > fst e1 /\ ord e e1 a <==> 
+                                           mem e b /\ mem e1 b /\ fst e > fst e1 /\ ord e e1 b))
 let convergence1 tr a b = ()
 
 val remove_id : id:nat 
@@ -222,11 +204,11 @@ val lem_same : a:s -> b:s
              -> Lemma (requires (forall e. mem e a <==> mem e b) /\
                                (forall id. mem_id_s id a <==> mem_id_s id b) /\
                                (List.Tot.length a = List.Tot.length b) /\
-                               (forall e e1. mem e a /\ mem e1 a /\ fst e <> fst e1 /\ ord e e1 a /\ fst e > fst e1 <==> 
-                                        mem e b /\ mem e1 b /\ fst e <> fst e1 /\ ord e e1 b /\ fst e > fst e1))
+                               (forall e e1. mem e a /\ mem e1 a /\ ord e e1 a /\ fst e > fst e1 <==> 
+                                        mem e b /\ mem e1 b /\ ord e e1 b /\ fst e > fst e1))
                      (ensures (forall e. mem e a /\ mem e b ==> pos e a = pos e b) /\ a = b)
 
-#set-options "--z3rlimit 10000000"
+#set-options "--z3rlimit 1000"
 #set-options "--initial_fuel 10 --max_fuel 10 --initial_ifuel 10 --max_ifuel 10"
 let rec lem_same a b =
   match a,b with
@@ -237,15 +219,15 @@ let rec lem_same a b =
                       assert (length (x1::xs) = length (y1::ys));
                       assert (ord x x1 a /\ ord y y1 b /\ ord x x1 b /\ ord y y1 a);
                       assert (pos x a = pos y b /\ pos x1 a = pos y1 b);
-                      assert (forall e. mem e xs /\ fst x1 <> fst e /\ fst x1 > fst e /\ ord x1 e a <==> 
-                                   mem e ys /\ fst y1 <> fst e /\ fst y1 > fst e /\ ord y1 e b); 
+                      assert (forall e. mem e xs /\ fst x1 > fst e /\ ord x1 e a <==> 
+                                   mem e ys /\ fst y1 > fst e /\ ord y1 e b); 
                       assert (fst x <> fst x1 /\ fst y <> fst y1 /\ x = y /\ x1 = y1);
                       assert (forall e. mem e (x1::xs) <==> mem e (y1::ys)); 
-                      assert (forall e. mem e (x1::xs) /\ fst x <> fst e /\ fst x > fst e /\ ord x e a <==> 
-                                   mem e (y1::ys) /\ fst y <> fst e /\ fst x > fst e /\ ord y e b);
+                      assert (forall e. mem e (x1::xs) /\ fst x > fst e /\ ord x e a <==> 
+                                   mem e (y1::ys) /\ fst x > fst e /\ ord y e b);
                       assert (forall e. mem e xs <==> mem e ys /\ unique_s ys /\ total_order ys); 
-                      assert (forall e e1. mem e (x1::xs) /\ mem e1 (x1::xs) /\ fst e <> fst e1 /\ fst e > fst e1 /\ ord e e1 (x1::xs) <==>
-                                      mem e (y1::ys) /\ mem e1 (y1::ys) /\ fst e <> fst e1 /\ fst e > fst e1 /\ ord e e1 (y1::ys));
+                      assert (forall e e1. mem e (x1::xs) /\ mem e1 (x1::xs) /\ fst e > fst e1 /\ ord e e1 (x1::xs) <==>
+                                      mem e (y1::ys) /\ mem e1 (y1::ys) /\ fst e > fst e1 /\ ord e e1 (y1::ys));
                       lem_same (x1::xs) (y1::ys) 
 
 val convergence : tr:ae op
@@ -265,11 +247,11 @@ val union_s : a:s
               (requires (forall e. mem e a ==> not (mem_id_s (fst e) b)) /\ 
                         (forall e. mem e b ==> not (mem_id_s (fst e) a)))
               (ensures (fun u -> (forall e. mem e u <==> mem e a \/ mem e b)/\
-                              (forall e e1. ((mem e a /\ mem e1 a /\ fst e <> fst e1 /\ fst e > fst e1 /\ ord e e1 a) \/
-                              (mem e b /\ mem e1 b /\ fst e <> fst e1 /\ fst e > fst e1 /\ ord e e1 b) \/
-                              (mem e a /\ mem e1 b /\ fst e <> fst e1 /\ fst e > fst e1) \/
-                              (mem e b /\ mem e1 a /\ fst e <> fst e1 /\ fst e > fst e1)) <==>
-                              (mem e u /\ mem e1 u /\ fst e <> fst e1 /\ fst e > fst e1 /\ ord e e1 u)) /\
+                              (forall e e1. ((mem e a /\ mem e1 a /\ fst e > fst e1 /\ ord e e1 a) \/
+                              (mem e b /\ mem e1 b /\ fst e > fst e1 /\ ord e e1 b) \/
+                              (mem e a /\ mem e1 b /\ fst e > fst e1) \/
+                              (mem e b /\ mem e1 a /\ fst e > fst e1)) <==>
+                              (mem e u /\ mem e1 u /\ fst e > fst e1 /\ ord e e1 u)) /\
                               (forall id. mem_id_s id u <==> mem_id_s id a \/ mem_id_s id b)))
 
 #set-options "--z3rlimit 10000000"
@@ -285,8 +267,8 @@ val remove : x:(nat * string)
            -> Pure s (requires (mem x a))
                     (ensures (fun r -> (forall e. mem e r <==> mem e a /\ e <> x) /\ not (mem_id_s (fst x) r) /\
                                     (forall id. mem_id_s id r <==> mem_id_s id a /\ id <> fst x) /\
-                                    (forall e e1. mem e r /\ mem e1 r /\ fst e <> fst e1 /\ fst e > fst e1 /\ ord e e1 r <==>
-                           mem e a /\ mem e1 a /\ fst e <> fst e1 /\ fst e > fst e1 /\ ord e e1 a /\ e <> x /\ e1 <> x)))
+                                    (forall e e1. mem e r /\ mem e1 r /\ fst e > fst e1 /\ ord e e1 r <==>
+                           mem e a /\ mem e1 a /\ fst e > fst e1 /\ ord e e1 a /\ e <> x /\ e1 <> x)))
 let rec remove x a =
   match a with
   |x1::xs -> if x = x1 then xs else x1::(remove x xs)
@@ -296,8 +278,8 @@ val diff_s : a:s -> l:s
              (requires (forall e. mem e l ==> mem e a))
              (ensures (fun r -> (forall e. mem e r <==> mem e a /\ not (mem e l)) /\
                              (forall id. mem_id_s id r <==> mem_id_s id a /\ not (mem_id_s id l)) /\
-                             (forall e e1. mem e r /\ mem e1 r /\ fst e <> fst e1 /\ fst e > fst e1 /\ ord e e1 r <==>
-             mem e a /\ mem e1 a /\ not (mem e l) /\ not (mem e1 l) /\ fst e <> fst e1 /\ fst e > fst e1 /\ ord e e1 a)))
+                             (forall e e1. mem e r /\ mem e1 r /\ fst e > fst e1 /\ ord e e1 r <==>
+             mem e a /\ mem e1 a /\ not (mem e l) /\ not (mem e1 l) /\ fst e > fst e1 /\ ord e e1 a)))
              (decreases l)
 let rec diff_s a l = 
   match l with
@@ -305,11 +287,11 @@ let rec diff_s a l =
   |x::xs -> diff_s (remove x a) xs
 
 val pre_cond_merge : l:s
-                    -> a:s
-                    -> b:s
-                    -> Tot (b1:bool {b1 = true <==> (forall e. mem e l <==> mem e a /\ mem e b) /\
-                                                 (forall e. mem e (diff_s a l) ==> not (mem_id_s (fst e) (diff_s b l))) /\
-                                                 (forall e. mem e (diff_s b l) ==> not (mem_id_s (fst e) (diff_s a l)))})
+                   -> a:s
+                   -> b:s
+                   -> Tot (b1:bool {b1 = true <==> (forall e. mem e l <==> mem e a /\ mem e b) /\
+                                     (forall e. mem e (diff_s a l) ==> not (mem_id_s (fst e) (diff_s b l))) /\
+                                                (forall e. mem e (diff_s b l) ==> not (mem_id_s (fst e) (diff_s a l)))})
 let pre_cond_merge l a b = 
   forallb (fun e -> mem e a && mem e b) l &&
   forallb (fun e -> not (mem_id_s (fst e) (diff_s b l))) (diff_s a l) &&
@@ -321,18 +303,18 @@ val merge : l:s
            -> Pure s
              (requires pre_cond_merge l a b)
              (ensures (fun r -> (forall e. mem e r <==> mem e a \/ mem e b) /\
-                           (forall e e1. (mem e r /\ mem e1 r /\ fst e <> fst e1 /\ fst e > fst e1 /\ ord e e1 r) <==>
-                           (mem e l /\ mem e1 l /\ fst e <> fst e1 /\ fst e > fst e1 /\ ord e e1 l) \/
-             (mem e (diff_s a l) /\ mem e1 (diff_s a l) /\ fst e <> fst e1 /\ fst e > fst e1 /\ ord e e1 (diff_s a l)) \/
-             (mem e (diff_s b l) /\ mem e1 (diff_s b l) /\ fst e <> fst e1 /\ fst e > fst e1 /\ ord e e1 (diff_s b l)) \/
-             (mem e (diff_s a l) /\ mem e1 (diff_s b l) /\ fst e <> fst e1 /\ fst e > fst e1) \/
-             (mem e (diff_s b l) /\ mem e1 (diff_s a l) /\ fst e <> fst e1 /\ fst e > fst e1) \/
-             (mem e (diff_s a l) /\ mem e1 l /\ fst e <> fst e1 /\ fst e > fst e1) \/
-             (mem e (diff_s b l) /\ mem e1 l /\ fst e <> fst e1 /\ fst e > fst e1) \/
-             (mem e l /\ mem e1 (diff_s a l) /\ fst e <> fst e1 /\ fst e > fst e1) \/
-             (mem e l /\ mem e1 (diff_s b l) /\ fst e <> fst e1 /\ fst e > fst e1))))
+                           (forall e e1. (mem e r /\ mem e1 r /\ fst e > fst e1 /\ ord e e1 r) <==>
+                           (mem e l /\ mem e1 l /\ fst e > fst e1 /\ ord e e1 l) \/
+             (mem e (diff_s a l) /\ mem e1 (diff_s a l) /\ fst e > fst e1 /\ ord e e1 (diff_s a l)) \/
+             (mem e (diff_s b l) /\ mem e1 (diff_s b l) /\ fst e > fst e1 /\ ord e e1 (diff_s b l)) \/
+             (mem e (diff_s a l) /\ mem e1 (diff_s b l) /\ fst e > fst e1) \/
+             (mem e (diff_s b l) /\ mem e1 (diff_s a l) /\ fst e > fst e1) \/
+             (mem e (diff_s a l) /\ mem e1 l /\ fst e > fst e1) \/
+             (mem e (diff_s b l) /\ mem e1 l /\ fst e > fst e1) \/
+             (mem e l /\ mem e1 (diff_s a l) /\ fst e > fst e1) \/
+             (mem e l /\ mem e1 (diff_s b l) /\ fst e > fst e1))))
 
-#set-options "--z3rlimit 10000000"
+#set-options "--z3rlimit 1000"
 let merge l a b = 
   let la = diff_s a l in
   let lb = diff_s b l in
@@ -352,25 +334,24 @@ val prop_merge : ltr:ae op
                                  (forall e. mem e atr.l ==> not (mem_id (get_id e) btr.l)) /\
                                  (forall e. mem e ltr.l ==> not (mem_id (get_id e) btr.l)) /\
                                  (sim ltr l /\ sim (union ltr atr) a /\ sim (union ltr btr) b))
-                       (ensures (sim (absmerge ltr atr btr) (merge l a b)))
+                       (ensures (pre_cond_merge l a b) /\ (sim (abs_merge ltr atr btr) (merge l a b)))
 
-#set-options "--z3rlimit 10000000"
+#set-options "--z3rlimit 1000"
 let prop_merge ltr l atr a btr b = 
   let m = merge l a b in
   assert (forall e. mem e m <==> mem e a \/ mem e b); 
-  assert (forall e e1. (mem e m /\ mem e1 m /\ fst e <> fst e1 /\ fst e > fst e1 /\ ord e e1 m) <==>
-                  (mem e a /\ mem e1 a /\ fst e <> fst e1 /\ fst e > fst e1 /\ ord e e1 a) \/
-                  (mem e b /\ mem e1 b /\ fst e <> fst e1 /\ fst e > fst e1 /\ ord e e1 b) \/
-                  (mem e a /\ mem e1 b /\ fst e <> fst e1 /\ fst e > fst e1) \/
-                  (mem e b /\ mem e1 a /\ fst e <> fst e1 /\ fst e > fst e1));
-  assert (forall e. mem e m <==> mem (fst e, (Append (snd e))) (absmerge ltr atr btr).l);
-  assert (forall e e1. (mem e m /\ mem e1 m /\ fst e <> fst e1 /\ fst e > fst e1 /\ ord e e1 m) ==>
-                mem (fst e, (Append (snd e))) (absmerge ltr atr btr).l /\ 
-                mem (fst e1, (Append (snd e1))) (absmerge ltr atr btr).l /\ fst e <> fst e1 /\ fst e > fst e1);
-  assert (forall e e1. mem e (absmerge ltr atr btr).l /\ mem e1 (absmerge ltr atr btr).l /\ 
-                  get_id e <> get_id e1 /\ get_id e > get_id e1 ==> 
+  assert (forall e e1. (mem e m /\ mem e1 m /\ fst e > fst e1 /\ ord e e1 m) <==>
+                  (mem e a /\ mem e1 a /\ fst e > fst e1 /\ ord e e1 a) \/
+                  (mem e b /\ mem e1 b /\ fst e > fst e1 /\ ord e e1 b) \/
+                  (mem e a /\ mem e1 b /\ fst e > fst e1) \/
+                  (mem e b /\ mem e1 a /\ fst e > fst e1));
+  assert (forall e. mem e m <==> mem (fst e, (Append (snd e))) (abs_merge ltr atr btr).l);
+  assert (forall e e1. (mem e m /\ mem e1 m /\ fst e > fst e1 /\ ord e e1 m) ==>
+                mem (fst e, (Append (snd e))) (abs_merge ltr atr btr).l /\ 
+                mem (fst e1, (Append (snd e1))) (abs_merge ltr atr btr).l /\ fst e > fst e1);
+  assert (forall e e1. mem e (abs_merge ltr atr btr).l /\ mem e1 (abs_merge ltr atr btr).l /\ get_id e > get_id e1 ==> 
                   mem (get_id e, get_msg e) m /\ mem (get_id e1, get_msg e1) m /\
-                  get_id e <> get_id e1 /\ get_id e > get_id e1 /\ ord (get_id e, get_msg e) (get_id e1, get_msg e1) m);
+                  get_id e > get_id e1 /\ ord (get_id e, get_msg e) (get_id e1, get_msg e1) m);
   ()
 
 val prop_spec1 : tr:ae op
@@ -378,19 +359,17 @@ val prop_spec1 : tr:ae op
               -> op:(nat * op)
               -> Lemma (requires (sim tr st) /\ (not (mem_id (get_id op) tr.l)) /\ not (opa op) /\
                                 (forall e. mem e tr.l ==> get_id e < get_id op) /\ get_id op > 0)
-                      (ensures (get_rval (app_op st op) = (spec op tr)))
-#set-options "--z3rlimit 1000000"
+                      (ensures (get_rval (do st op) = (spec op tr)))
 let prop_spec1 tr st op = 
-  lem_length (extract (get_rval (app_op st op))) (extract (spec op tr));
-  lem_same (extract (get_rval (app_op st op))) (extract (spec op tr))
+  lem_length (extract (get_rval (do st op))) (extract (spec op tr));
+  lem_same (extract (get_rval (do st op))) (extract (spec op tr))
 
 val prop_spec : tr:ae op
               -> st:s
               -> op:(nat * op)
               -> Lemma (requires (sim tr st) /\ (not (mem_id (get_id op) tr.l)) /\
                                 (forall e. mem e tr.l ==> get_id e < get_id op) /\ get_id op > 0)
-                      (ensures (get_rval (app_op st op) = (spec op tr)))
-#set-options "--z3rlimit 1000000"
+                      (ensures (get_rval (do st op) = (spec op tr)))
 let prop_spec tr st op = 
   if not (opa op) then prop_spec1 tr st op else ()
 
@@ -398,13 +377,13 @@ instance log : mrdt s op rval = {
   Library.init = init;
   Library.spec = spec;
   Library.sim = sim;
-  Library.pre_cond_app_op = pre_cond_app_op;
-  Library.pre_cond_prop_oper = pre_cond_prop_oper;
+  Library.pre_cond_do = pre_cond_do;
+  Library.pre_cond_prop_do = pre_cond_prop_do;
   Library.pre_cond_merge = pre_cond_merge;
   Library.pre_cond_prop_merge = pre_cond_prop_merge;
-  Library.app_op = app_op;
+  Library.do = do;
   Library.merge = merge;
-  Library.prop_oper = prop_oper;
+  Library.prop_do = prop_do;
   Library.prop_merge = prop_merge;
   Library.prop_spec = prop_spec;
   Library.convergence = convergence
