log_map.fst
@@ -1,8 +1,9 @@
 module Log_map
 open FStar.List.Tot
 
+#set-options "--query_stats"
+
 open Library
-open FStar.Tactics.Typeclasses
 
 module A = Alpha_map
 
@@ -17,7 +18,7 @@ val pre_cond_merge_a1 : l:A.s G.s -> a:A.s G.s -> b:A.s G.s
                         (forall e e1. mem e (A.get_val_s #G.s #G.op #G.rval ch l) /\ mem e1 (G.diff_s (A.get_val_s #G.s #G.op #G.rval ch a) (A.get_val_s #G.s #G.op #G.rval ch l)) ==> G.fst e1 > G.fst e) /\
                         (forall e e1. mem e (A.get_val_s #G.s #G.op #G.rval ch l) /\ mem e1 (G.diff_s (A.get_val_s #G.s #G.op #G.rval ch b) (A.get_val_s #G.s #G.op #G.rval ch l)) ==> G.fst e1 > G.fst e)))))
 
-#set-options "--z3rlimit 10000000"
+#set-options "--z3rlimit 1000"
 let pre_cond_merge_a1 l a b = 
   forallb (fun e -> A.mem_key_s (A.get_key_s #G.s e) a && A.mem_key_s (A.get_key_s #G.s e) b) l &&
   forallb (fun ch -> (forallb (fun e -> mem e (A.get_val_s #G.s #G.op #G.rval ch a) && mem e (A.get_val_s #G.s #G.op #G.rval ch b)) (A.get_val_s #G.s #G.op #G.rval ch l)) &&
@@ -36,7 +37,7 @@ val pre_cond_merge_a2 : l:A.s G.s -> a:A.s G.s -> b:A.s G.s
             (forall e. mem e (G.diff_s (A.get_val_s #G.s #G.op #G.rval ch b) (A.get_val_s #G.s #G.op #G.rval ch l)) ==>
                            not (G.mem_id_s (G.fst e) (G.diff_s (A.get_val_s #G.s #G.op #G.rval ch a) (A.get_val_s#G.s #G.op #G.rval ch l))))))))
 
-#set-options "--z3rlimit 10000000"
+#set-options "--z3rlimit 1000"
 let pre_cond_merge_a2 l a b =
   forallb (fun ch -> G.pre_cond_merge (A.get_val_s #G.s #G.op #G.rval ch l) (A.get_val_s #G.s #G.op #G.rval ch a) (A.get_val_s #G.s #G.op #G.rval ch b) &&
   (forallb (fun e -> mem e (A.get_val_s #G.s #G.op #G.rval ch a) && mem e (A.get_val_s #G.s #G.op #G.rval ch b)) (A.get_val_s #G.s #G.op #G.rval ch l)) &&
@@ -58,7 +59,6 @@ val pre_cond_merge_a : l:A.s G.s -> a:A.s G.s -> b:A.s G.s
             (forall e e1. mem e (A.get_val_s #G.s #G.op #G.rval ch l) /\ mem e1 (G.diff_s (A.get_val_s #G.s #G.op #G.rval ch a) (A.get_val_s #G.s #G.op #G.rval ch l)) ==> G.fst e1 > G.fst e) /\
             (forall e e1. mem e (A.get_val_s #G.s #G.op #G.rval ch l) /\ mem e1 (G.diff_s (A.get_val_s #G.s #G.op #G.rval ch b) (A.get_val_s #G.s #G.op #G.rval ch l)) ==> G.fst e1 > G.fst e)))))
 
-#set-options "--z3rlimit 10000000"
 let pre_cond_merge_a l a b =
   pre_cond_merge_a1 l a b &&
   pre_cond_merge_a2 l a b
@@ -92,16 +92,16 @@ val lemma1 : tr:ae (A.op G.op)
          -> op1:(nat * (A.op G.op))
          -> Lemma (requires (A.sim_a #G.s #G.op #G.rval tr st) /\ (not (mem_id (get_id op1) tr.l)) /\
                            (forall e. mem e tr.l ==> get_id e < get_id op1) /\ get_id op1 > 0 /\
-                          G.pre_cond_app_op (A.get_val_s #G.s #G.op #G.rval (A.get_key op1) st) (A.project_op op1))
-                 (ensures (forall i. A.mem_key_s i (get_st (A.app_op_a #G.s #G.op #G.rval st op1)) /\ i <> A.get_key op1 ==>
-                 ((forall e. mem e (A.project i (append tr op1)).l <==> mem e (A.project i tr).l) /\
-             (forall e e1. mem e (A.project i (append tr op1)).l /\ mem e1 (A.project i (append tr op1)).l /\ get_id e <> get_id e1 /\
-                      (A.project i (append tr op1)).vis e e1 <==> 
+                          G.pre_cond_do (A.get_val_s #G.s #G.op #G.rval (A.get_key op1) st) (A.project_op op1))
+                 (ensures (forall i. A.mem_key_s i (get_st (A.do_a #G.s #G.op #G.rval st op1)) /\ i <> A.get_key op1 ==>
+                 ((forall e. mem e (A.project i (abs_do tr op1)).l <==> mem e (A.project i tr).l) /\
+             (forall e e1. mem e (A.project i (abs_do tr op1)).l /\ mem e1 (A.project i (abs_do tr op1)).l /\ get_id e <> get_id e1 /\
+                      (A.project i (abs_do tr op1)).vis e e1 <==> 
                  mem e (A.project i tr).l /\ mem e1 (A.project i tr).l /\ get_id e <> get_id e1 /\ (A.project i tr).vis e e1) /\
-             (A.get_val_s #G.s #G.op #G.rval i (get_st (A.app_op_a #G.s #G.op #G.rval st op1)) = (A.get_val_s #G.s #G.op #G.rval i st))) ==>
-                          (G.sim (A.project i (append tr op1)) (A.get_val_s #G.s #G.op #G.rval i (get_st (A.app_op_a #G.s #G.op #G.rval st op1))))))
+             (A.get_val_s #G.s #G.op #G.rval i (get_st (A.do_a #G.s #G.op #G.rval st op1)) = (A.get_val_s #G.s #G.op #G.rval i st))) ==>
+                          (G.sim (A.project i (abs_do tr op1)) (A.get_val_s #G.s #G.op #G.rval i (get_st (A.do_a #G.s #G.op #G.rval st op1))))))
 
-#set-options "--z3rlimit 10000000"
+#set-options "--z3rlimit 1000"
 let lemma1 tr st op = ()
 
 val lemma7 : tr:ae G.op -> s1:G.s -> tr1:ae G.op
@@ -109,7 +109,7 @@ val lemma7 : tr:ae G.op -> s1:G.s -> tr1:ae G.op
                              (forall e e1. mem e tr1.l /\ mem e1 tr1.l /\ get_id e <> get_id e1 /\ tr1.vis e e1 <==>
                                       mem e tr.l /\ mem e1 tr.l /\ get_id e <> get_id e1 /\ tr.vis e e1))
                    (ensures (G.sim tr1 s1))
-#set-options "--z3rlimit 10000000"
+#set-options "--z3rlimit 1000"
 let lemma7 tr s1 tr1 = ()
 
 instance _ : A.alpha_map G.s G.op G.rval G.log = {
@@ -147,41 +147,41 @@ let pre_cond_prop_merge_a ltr l atr a btr b =
   (G.sim (union (A.project ch ltr) (A.project ch atr)) (A.get_val_s #G.s #G.op #G.rval ch a)) &&
   (G.sim (union (A.project ch ltr) (A.project ch btr)) (A.get_val_s #G.s #G.op #G.rval ch b))) (A.get_key_lst l a b)
 
-val pre_cond_app_op_a : s1:(A.s G.s) -> op1:(nat * (A.op G.op))
-                    -> Tot (b:bool {b = true <==> 
-                          G.pre_cond_app_op (A.get_val_s #G.s #G.op #G.rval (A.get_key op1) s1) (A.project_op op1)})
-let pre_cond_app_op_a s1 op = 
-      G.pre_cond_app_op (A.get_val_s #G.s #G.op #G.rval (A.get_key op) s1) (A.project_op op)
+val pre_cond_do_a : s1:(A.s G.s) -> op1:(nat * (A.op G.op))
+                  -> Tot (b:bool {b = true <==> 
+                        G.pre_cond_do (A.get_val_s #G.s #G.op #G.rval (A.get_key op1) s1) (A.project_op op1)})
+let pre_cond_do_a s1 op = 
+  G.pre_cond_do (A.get_val_s #G.s #G.op #G.rval (A.get_key op) s1) (A.project_op op)
 
-val pre_cond_prop_oper_a : tr:ae (A.op G.op)
-                         -> st:(A.s G.s)
-                         -> op1:(nat * (A.op G.op)) 
-                         -> Pure bool
-                           (requires (not (mem_id (get_id op1) tr.l) /\
-                                     (forall e. mem e tr.l ==> get_id e < get_id op1) /\ get_id op1 > 0))
-                           (ensures (fun b -> (b=true <==> (G.pre_cond_prop_oper (A.project (A.get_key op1) (append tr op1))
-                                    (A.get_val_s #G.s #G.op #G.rval (A.get_key op1) st) (A.project_op op1)) /\
-                                    G.pre_cond_app_op (A.get_val_s #G.s #G.op #G.rval (A.get_key op1) st) (A.project_op op1) /\
-                           (G.sim (A.project (A.get_key op1) (append tr op1)) (A.get_val_s #G.s #G.op #G.rval (A.get_key op1) (get_st (A.app_op_a #G.s #G.op #G.rval st op1)))))))
+val pre_cond_prop_do_a : tr:ae (A.op G.op)
+                       -> st:(A.s G.s)
+                       -> op1:(nat * (A.op G.op)) 
+                       -> Pure bool
+                         (requires (not (mem_id (get_id op1) tr.l) /\
+                                   (forall e. mem e tr.l ==> get_id e < get_id op1) /\ get_id op1 > 0))
+                         (ensures (fun b -> (b=true <==> (G.pre_cond_prop_do (A.project (A.get_key op1) (abs_do tr op1))
+                                  (A.get_val_s #G.s #G.op #G.rval (A.get_key op1) st) (A.project_op op1)) /\
+                              G.pre_cond_do (A.get_val_s #G.s #G.op #G.rval (A.get_key op1) st) (A.project_op op1) /\
+                           (G.sim (A.project (A.get_key op1) (abs_do tr op1)) (A.get_val_s #G.s #G.op #G.rval (A.get_key op1) (get_st (A.do_a #G.s #G.op #G.rval st op1)))))))
 
-let pre_cond_prop_oper_a tr st op1 =
-    G.pre_cond_prop_oper (A.project (A.get_key op1) (append tr op1))
+let pre_cond_prop_do_a tr st op1 =
+    G.pre_cond_prop_do (A.project (A.get_key op1) (abs_do tr op1))
                          (A.get_val_s #G.s #G.op #G.rval (A.get_key op1) st) (A.project_op op1) &&
-    G.pre_cond_app_op (A.get_val_s #G.s #G.op #G.rval (A.get_key op1) st) (A.project_op op1) &&
-    G.sim (A.project (A.get_key op1) (append tr op1)) (A.get_val_s #G.s #G.op #G.rval (A.get_key op1) 
-                     (get_st (A.app_op_a #G.s #G.op #G.rval st op1)))
+    G.pre_cond_do (A.get_val_s #G.s #G.op #G.rval (A.get_key op1) st) (A.project_op op1) &&
+    G.sim (A.project (A.get_key op1) (abs_do tr op1)) (A.get_val_s #G.s #G.op #G.rval (A.get_key op1) 
+                     (get_st (A.do_a #G.s #G.op #G.rval st op1)))
 
-val prop_oper_a : tr:ae (A.op G.op)
+val prop_do_a : tr:ae (A.op G.op)
               -> st:A.s G.s
               -> op1:(nat * (A.op G.op)) 
               -> Lemma (requires (A.sim_a #G.s #G.op #G.rval tr st) /\ (not (mem_id (get_id op1) tr.l)) /\
                                 (forall e. mem e tr.l ==> get_id e < get_id op1) /\ get_id op1 > 0 /\
-                                pre_cond_app_op_a st op1 /\ pre_cond_prop_oper_a tr st op1)
-                      (ensures (A.sim_a #G.s #G.op #G.rval (append tr op1) (get_st (A.app_op_a #G.s #G.op #G.rval st op1))))
+                                pre_cond_do_a st op1 /\ pre_cond_prop_do_a tr st op1)
+                      (ensures (A.sim_a #G.s #G.op #G.rval (abs_do tr op1) (get_st (A.do_a #G.s #G.op #G.rval st op1))))
 
-#set-options "--z3rlimit 10000000"
-let prop_oper_a tr st op = 
-  A.prop_oper_a #G.s #G.op #G.rval #G.log tr st op
+#set-options "--z3rlimit 1000"
+let prop_do_a tr st op = 
+  A.prop_do_a #G.s #G.op #G.rval #G.log tr st op
 
 val convergence2 : tr:ae (A.op G.op)
                  -> a:(A.s G.s)
@@ -195,7 +195,7 @@ val convergence2 : tr:ae (A.op G.op)
           (forall ch. A.mem_key_s ch a /\ A.mem_key_s ch b ==>
     (forall e. G.mem_id_s e (A.get_val_s #G.s #G.op #G.rval ch a) <==> G.mem_id_s e (A.get_val_s #G.s #G.op #G.rval ch b))))
 
-#set-options "--z3rlimit 100000000"
+#set-options "--z3rlimit 1000"
 let convergence2 tr a b = 
   A.convergence_a1 #G.s #G.op #G.rval tr a b
 
@@ -232,7 +232,7 @@ val convergence3 : a:(A.s G.s)
                           (ensures (forall ch. mem ch lst ==> (A.get_val_s #G.s #G.op #G.rval ch a = 
                                                          A.get_val_s #G.s #G.op #G.rval ch b)))
                          (decreases lst)
-#set-options "--z3rlimit 10000000"
+#set-options "--z3rlimit 10000"
 let rec convergence3 a b lst =
   match lst with
   |[] -> ()
@@ -247,7 +247,7 @@ val convergence_a : tr:ae (A.op G.op)
                                    (forall ch. A.mem_key_s ch a /\ A.mem_key_s ch b ==> 
                                    (A.get_val_s #G.s #G.op #G.rval ch a) = (A.get_val_s #G.s #G.op #G.rval ch b)))
 
-#set-options "--z3rlimit 100000000"
+#set-options "--z3rlimit 1000"
 let convergence_a tr a b = 
   A.convergence_a1 #G.s #G.op #G.rval  tr a b;
   convergence2 tr a b;
@@ -273,9 +273,9 @@ val prop_merge_a : ltr:ae (A.op G.op)
                             (forall e. mem e (A.project ch atr).l ==> not (mem_id (get_id e) (A.project ch btr).l)) /\
                             (forall e. mem e (A.project ch ltr).l ==> not (mem_id (get_id e) (A.project ch btr).l)) /\
                 (sim #G.s #G.op #G.rval (A.project ch ltr) (A.get_val_s #G.s #G.op #G.rval ch l) /\ sim #G.s #G.op #G.rval (union (A.project ch ltr) (A.project ch atr)) (A.get_val_s #G.s #G.op #G.rval ch a) /\ sim #G.s #G.op #G.rval (union (A.project ch ltr) (A.project ch btr)) (A.get_val_s #G.s #G.op #G.rval ch b))))
-                (ensures (A.sim_a #G.s #G.op #G.rval (absmerge ltr atr btr) (merge_a l a b)))
+                (ensures (A.sim_a #G.s #G.op #G.rval (abs_merge ltr atr btr) (merge_a l a b)))
 
-#set-options "--z3rlimit 10000000"
+#set-options "--z3rlimit 1000"
 let prop_merge_a ltr l atr a btr b = 
   A.prop_merge_a #G.s #G.op #G.rval #G.log ltr l atr a btr b
 
@@ -294,11 +294,11 @@ val prop_spec_a : tr:ae (A.op G.op)
                   -> op:(nat * (A.op G.op))
                   -> Lemma (requires (A.sim_a #G.s #G.op #G.rval tr st1) /\ (not (mem_id (get_id op) tr.l)) /\
                                     (forall e. mem e tr.l ==> get_id e < get_id op) /\ get_id op > 0 /\
-                                    pre_cond_app_op_a st1 op)
-                    (ensures A.opget op ==> (get_rval (A.app_op_a #G.s #G.op #G.rval st1 op)) =
+                                    pre_cond_do_a st1 op)
+                    (ensures A.opget op ==> (get_rval (A.do_a #G.s #G.op #G.rval st1 op)) =
                                                   ((A.spec_a #G.s #G.op #G.rval) op tr))
 
-#set-options "--z3rlimit 1000000"
+#set-options "--z3rlimit 1000"
 let prop_spec_a tr st op =
   G.prop_spec (A.project (A.get_key op) tr) (A.get_val_s #G.s #G.op #G.rval (A.get_key op) st) (A.project_op op)
 
@@ -309,18 +309,17 @@ val sim_a : tr:ae (A.op G.op)
               (forall e. mem e tr.l /\ A.opset e ==> (exists e1. mem e1 s1 /\ A.get_key e = A.get_key_s e1))})
 let sim_a tr s1 = A.sim_a #G.s #G.op #G.rval tr s1
 
-#set-options "--z3rlimit 10000000" 
 instance log_map : mrdt (A.s G.s) (A.op G.op) (G.rval) = {
   Library.init = A.init_a;
   Library.spec = spec_a;
   Library.sim = sim_a;
-  Library.pre_cond_app_op = pre_cond_app_op_a;
-  Library.pre_cond_prop_oper = pre_cond_prop_oper_a;
+  Library.pre_cond_do = pre_cond_do_a;
+  Library.pre_cond_prop_do = pre_cond_prop_do_a;
   Library.pre_cond_merge = pre_cond_merge_a;
   Library.pre_cond_prop_merge = pre_cond_prop_merge_a;
-  Library.app_op = A.app_op_a;
+  Library.do = A.do_a;
   Library.merge = merge_a;
-  Library.prop_oper = prop_oper_a;
+  Library.prop_do = prop_do_a;
   Library.prop_merge = prop_merge_a;
   Library.prop_spec = prop_spec_a;
   Library.convergence = convergence_a
