lww.fst
@@ -1,6 +1,8 @@
 module Lww
 open FStar.List.Tot
 
+#set-options "--query_stats"
+
 open Library
 
 type s = (nat (*timestamp*) * nat (*value*))
@@ -28,12 +30,12 @@ let get_id_s (t, v) = t
 val get_ele_s : s -> nat
 let get_ele_s (t, v) = v
 
-let pre_cond_app_op s1 op = true
-let pre_cond_prop_oper tr s1 op = true
+let pre_cond_do s1 op = true
+let pre_cond_prop_do tr s1 op = true
 
-val app_op : s1:s -> op:(nat * op) -> Tot (s2:(s * rval) {(opw op ==> s2 = (((get_id op), (get_val op)), Bot)) /\
-                                                      (opr op ==> s2 = (s1, Val (get_ele_s s1)))})
-let app_op s1 o =
+val do : s1:s -> op:(nat * op) -> Tot (s2:(s * rval) {(opw op ==> s2 = (((get_id op), (get_val op)), Bot)) /\
+                                                  (opr op ==> s2 = (s1, Val (get_ele_s s1)))})
+let do s1 o =
   match o with
   |(t, Write n) -> ((t, n), Bot)
   |(_, Rd) -> (s1, Val (get_ele_s s1))
@@ -57,7 +59,6 @@ val gt : l:list (nat * op)
          (ensures (fun r -> (mem ((get_id_s r), Write (get_ele_s r)) l \/ r = init1) /\
                          (forall e. mem e l /\ opw e ==> get_id_s r >= get_id e) /\ (get_id_s r >= get_id_s init1)))
          (decreases (length l))
-#set-options "--z3rlimit 10000"
 let rec gt l init1 =
   match l with
   |[] -> init1
@@ -80,7 +81,6 @@ let spec o tr =
     |(_, Write _) -> Bot
     |(_, Rd) -> Val (snd (gt tr.l init))
 
-#set-options "--query_stats"
 val sim : tr:ae op
         -> s1:s
         -> Tot (b:bool {b = true <==> s1 = gt tr.l init} )
@@ -91,11 +91,11 @@ let pre_cond_merge l a b = true
 let pre_cond_prop_merge ltr l atr a btr b = true
 
 val merge : l:s
-           -> a:s
-           -> b:s
-           -> Pure s (requires pre_cond_merge l a b)
-                    (ensures (fun r -> (get_id_s a >= get_id_s b ==> r = a) /\
-                                    (get_id_s a < get_id_s b ==> r = b)))
+          -> a:s
+          -> b:s
+          -> Pure s (requires pre_cond_merge l a b)
+                   (ensures (fun r -> (get_id_s a >= get_id_s b ==> r = a) /\
+                                   (get_id_s a < get_id_s b ==> r = b)))
 let merge l a b =
   if (get_id_s a >= get_id_s b) then a else b
 
@@ -119,28 +119,27 @@ val prop_merge : ltr:ae op
                                  (forall e. mem e atr.l ==> not (mem_id (get_id e) btr.l)) /\
                                  (forall e. mem e ltr.l ==> not (mem_id (get_id e) btr.l)) /\
                                  (sim ltr l /\ sim (union ltr atr) a /\ sim (union ltr btr) b))
-                        (ensures (sim (absmerge ltr atr btr) (merge l a b)))
+                        (ensures (sim (abs_merge ltr atr btr) (merge l a b)))
 
-#set-options "--z3rlimit 10000000"
-let prop_merge ltr l atr a btr b = 
-  lemma (absmerge ltr atr btr).l;
-  ()
+#set-options "--z3rlimit 1000"
+let prop_merge ltr l atr a btr b =
+  lemma (abs_merge ltr atr btr).l
 
 val prop_spec : tr:ae op
               -> st:s
               -> op:(nat * op)
               -> Lemma (requires (sim tr st) /\ (not (mem_id (get_id op) tr.l)) /\
                                 (forall e. mem e tr.l ==> get_id e < get_id op) /\ get_id op > 0)
-                      (ensures (get_rval (app_op st op) = spec op tr))
+                      (ensures (get_rval (do st op) = spec op tr))
 let prop_spec tr st op = ()
 
-val prop_oper : tr:ae op
-              -> st:s
-              -> op:(nat * op)
-              -> Lemma (requires (sim tr st) /\ (not (mem_id (get_id op) tr.l)) /\
-                                (forall e. mem e tr.l ==> get_id e < get_id op) /\ get_id op > 0)
-                      (ensures (sim (append tr op) (get_st (app_op st op))))
-let prop_oper tr st op = ()
+val prop_do : tr:ae op
+            -> st:s
+            -> op:(nat * op)
+            -> Lemma (requires (sim tr st) /\ (not (mem_id (get_id op) tr.l)) /\
+                              (forall e. mem e tr.l ==> get_id e < get_id op) /\ get_id op > 0)
+                    (ensures (sim (abs_do tr op) (get_st (do st op))))
+let prop_do tr st op = ()
 
 val convergence : tr:ae op
                 -> a:s
@@ -153,13 +152,13 @@ instance lww : mrdt s op rval = {
   Library.init = init;
   Library.spec = spec;
   Library.sim = sim;
-  Library.pre_cond_app_op = pre_cond_app_op;
-  Library.pre_cond_prop_oper = pre_cond_prop_oper;
+  Library.pre_cond_do = pre_cond_do;
+  Library.pre_cond_prop_do = pre_cond_prop_do;
   Library.pre_cond_merge = pre_cond_merge;
   Library.pre_cond_prop_merge = pre_cond_prop_merge;
-  Library.app_op = app_op;
+  Library.do = do;
   Library.merge = merge;
-  Library.prop_oper = prop_oper;
+  Library.prop_do = prop_do;
   Library.prop_merge = prop_merge;
   Library.prop_spec = prop_spec;
   Library.convergence = convergence
